sha/verif_sha_update4.v
@@ -1,0 +1,437 @@
+Require Import floyd.proofauto.
+Require Import sha.sha.
+Require Import sha.SHA256.
+Require Import sha.spec_sha.
+Require Import sha.sha_lemmas.
+Require Import sha.verif_sha_update2.
+Require Import sha.verif_sha_update3.
+Local Open Scope nat.
+Local Open Scope logic.
+
+
+Lemma Hblocks_lem:
+ forall {blocks: list int} {frag: list Z} {data},
+ intlist_to_Zlist blocks = frag ++ firstn (length blocks * 4 - length frag) data ->
+ length frag <= length blocks * 4.
+Proof.
+intros.
+assert (length (intlist_to_Zlist blocks) = 
+               length ( frag ++
+     firstn (length blocks * 4 - length frag) data)) by congruence.
+ rewrite length_intlist_to_Zlist, app_length in H0.
+ rewrite mult_comm; omega.
+Qed.
+
+Lemma intro_update_inv:
+ forall (len: nat) (blocks : list int) (frag data: list Z) (P' Q: Prop),
+  (forall (Hblocks_len: len >= length blocks * 4 - length frag)
+            (Hdiv: NPeano.divide LBLOCK (length blocks))
+            (Hblocks: intlist_to_Zlist blocks = frag ++ firstn (length blocks * 4 - length frag) data)
+            (DONE: P')
+            (Hblocks': length blocks * 4 >= length frag),
+            Q) ->
+    (len >= length blocks*4 - length frag /\
+    NPeano.divide LBLOCK (length blocks) /\ 
+    intlist_to_Zlist blocks = frag ++ firstn (length blocks * 4 - length frag) data /\
+              P' -> Q). 
+Proof.
+intros.
+ destruct H0 as  [Hblocks_len [Hdiv [Hblocks DONE]]].
+ apply H; clear H; auto.
+ apply Hblocks_lem in Hblocks; auto.
+Qed.
+
+Definition sha_update_loop_body :=
+  (Ssequence
+     (Scall None
+        (Evar _sha256_block_data_order
+           (Tfunction
+              (Tcons (tptr t_struct_SHA256state_st) (Tcons (tptr tvoid) Tnil))
+              tvoid))
+        [Etempvar _c (tptr t_struct_SHA256state_st),
+        Etempvar _data (tptr tuchar)])
+     (Ssequence
+        (Sset _data
+           (Ebinop Oadd (Etempvar _data (tptr tuchar))
+              (Ebinop Omul (Econst_int (Int.repr 16) tint)
+                 (Econst_int (Int.repr 4) tint) tint) (tptr tuchar)))
+        (Sset _len
+           (Ebinop Osub (Etempvar _len tuint)
+              (Ebinop Omul (Econst_int (Int.repr 16) tint)
+                 (Econst_int (Int.repr 4) tint) tint) tuint)))).
+
+Lemma update_loop_body_proof:
+ forall (Espec : OracleKind) (sh: share) (hashed : list int) (r_data data : list Z) (c d : val)
+  (len : nat) (r_h : list int) (r_Nl r_Nh : int)
+   (Delta : tycontext) (blocks bl : list int)
+ (HDelta: Delta = initialized _p (initialized _n (initialized _data
+                     (func_tycontext f_SHA256_Update Vprog Gtot))))
+ (H: len <= length data)
+ (Hdiv: NPeano.divide LBLOCK (length blocks))
+ (H0: r_h = process_msg init_registers hashed)
+ (H1: (Zlength (intlist_to_Zlist hashed ++ r_data)*8 = hilo r_Nh r_Nl)%Z)
+ (H4: NPeano.divide LBLOCK (length hashed))
+ (Hblocks: intlist_to_Zlist blocks =  r_data ++ firstn (length blocks * 4 - length r_data) data)
+ (H3 : length r_data < CBLOCK)
+ (Hlen: (Z.of_nat len <= Int.max_unsigned)%Z)
+ (Hlen_ge: len - (length blocks * 4 - length r_data) >= CBLOCK)
+ (H6: firstn CBLOCK (skipn (length blocks * 4 - length r_data) data) =
+     intlist_to_Zlist bl)
+ (H7: length bl = LBLOCK),
+semax Delta
+  (PROP  ()
+   LOCAL 
+   (`(typed_true
+        (typeof
+           (Ebinop Oge (Etempvar _len tuint)
+              (Ebinop Omul (Econst_int (Int.repr 16) tint)
+                 (Econst_int (Int.repr 4) tint) tint) tint)))
+      (eval_expr
+         (Ebinop Oge (Etempvar _len tuint)
+            (Ebinop Omul (Econst_int (Int.repr 16) tint)
+               (Econst_int (Int.repr 4) tint) tint) tint));
+   `(eq (offset_val (Int.repr 40) c)) (eval_id _p); `(eq c) (eval_id _c);
+   `(eq
+       (offset_val (Int.repr (Z.of_nat (length blocks * 4 - length r_data)))
+          d)) (eval_id _data);
+   `(eq
+       (Vint
+          (Int.repr (Z.of_nat (len - (length blocks * 4 - length r_data))))))
+     (eval_id _len))
+   SEP 
+   (K_vector;
+    `(array_at tuint Tsh
+        (tuints (process_msg init_registers (hashed ++ blocks))) 0 8 c);
+   `(sha256_length (hilo r_Nh r_Nl + (Z.of_nat len)*8) c);
+   `(array_at_ tuchar Tsh 0 64 (offset_val (Int.repr 40) c));
+   `(field_at_ Tsh t_struct_SHA256state_st _num c);
+   `(data_block sh data d)))
+   sha_update_loop_body
+  (loop1_ret_assert
+     (sha_update_inv sh hashed len c d r_data data r_Nh r_Nl false)
+     (normal_ret_assert
+        (sha_update_inv sh hashed len c d r_data data r_Nh r_Nl true))).
+Proof.
+intros.
+name c' _c.
+name data_ _data_.
+name len' _len.
+name data' _data.
+name p _p.
+name n _n.
+unfold sha_update_loop_body.
+subst Delta; simplify_Delta; abbreviate_semax.
+forward. (* sha256_block_data_order (c,data); *)
+instantiate (1:=(hashed++ blocks, 
+                           bl,
+                           c, 
+                           offset_val (Int.repr (Z.of_nat (length blocks * 4 - length r_data))) d,
+                           sh)) in (Value of witness).
+entailer!.
+rewrite mul_repr in H5; rewrite H5; reflexivity.
+apply divide_length_app; auto.
+unfold_lift.
+repeat rewrite eval_var_env_set.
+(*erewrite elim_globals_only by (split3; [eassumption | reflexivity.. ]). *)
+change (array_at tuint Tsh (tuints K) 0 (Zlength K)
+      (eval_var _K256 (tarray tuint 64) rho)) with (K_vector rho).
+ rewrite <- H6.
+ rewrite (split3_data_block (length blocks * 4 - length r_data) CBLOCK sh data) by omega.
+ cancel.
+
+replace_SEP 0%Z
+  (`(array_at tuint Tsh
+          (tuints
+             (process_msg init_registers ((hashed ++ blocks) ++ bl))) 0 8 c) *
+      `(data_block sh (intlist_to_Zlist bl)
+          (offset_val
+             (Int.repr (Z.of_nat (length blocks * 4 - length r_data))) d)) *
+      K_vector). {
+  entailer!.
+}
+ normalize.
+ forward. (* data += SHA_CBLOCK; *)
+ entailer.
+ forward. (* len  -= SHA_CBLOCK; *)
+ unfold loop1_ret_assert.
+ unfold sha_update_inv.
+ apply exp_right with (blocks++ bl).
+ entailer.
+ clear TC0 TC.
+ rewrite negb_true_iff in H8.
+ unfold Int.ltu in H8.
+ if_tac in H8; inv H8.
+ rewrite mul_repr in H0.
+ change (Int.unsigned (Int.repr (16 * 4)))%Z with 64%Z in H0.
+ rewrite Int.unsigned_repr in H0
+  by (clear - Hlen; split; [omega | ];
+        rewrite Nat2Z.inj_sub_max;
+        apply Z.max_lub; omega).
+
+ assert (Hblocks' := Hblocks_lem Hblocks).
+ apply andp_right; [ apply prop_right; repeat split | cancel].
+*
+ rewrite app_length.
+ rewrite  mult_plus_distr_r. 
+ rewrite plus_comm.
+ rewrite <- NPeano.Nat.add_sub_assoc by (clear - Hblocks'; omega).
+ rewrite H7.
+ clear - H0.
+ rewrite Nat2Z.inj_sub_max in H0.
+ rewrite Zmax_spec in H0. if_tac in H0; try omega.
+ clear H.
+ apply Nat2Z.inj_ge.
+ rewrite Nat2Z.inj_add.
+ change (Z.of_nat (LBLOCK*4)) with 64%Z. omega.
+* rewrite app_length.
+ clear - Hdiv H7. rewrite H7. destruct Hdiv as [x ?]; exists (S x).
+ simpl; omega.
+*
+ rewrite intlist_to_Zlist_app.
+ rewrite Hblocks; rewrite <- H6.
+ rewrite app_ass.
+ f_equal. rewrite app_length. rewrite H7.
+  rewrite  mult_plus_distr_r. change (LBLOCK*4)%nat with CBLOCK.
+ rewrite NPeano.Nat.add_sub_swap by auto.
+ apply firstn_app.
+*
+ destruct d; inv Pd; simpl. f_equal.
+  f_equal.
+ rewrite app_length.
+ rewrite H7.
+ f_equal.
+ rewrite  mult_plus_distr_r.
+ change (LBLOCK*4)%nat with CBLOCK.
+rewrite NPeano.Nat.add_sub_swap by auto.
+ rewrite Nat2Z.inj_add.
+ reflexivity.
+*
+ f_equal.
+ rewrite app_length. rewrite mult_plus_distr_r. rewrite H7.
+ change (16*4)%Z with  (Z.of_nat (LBLOCK*4)).
+ symmetry.  rewrite <- Nat2Z.inj_sub by auto.
+ f_equal.
+ rewrite <- NPeano.Nat.sub_add_distr by auto.
+ f_equal.
+ rewrite NPeano.Nat.add_sub_swap by auto.
+ auto.
+*
+ rewrite app_ass.
+ rewrite (split3_data_block (length blocks * 4 - length r_data) CBLOCK sh data)
+  by omega.
+ cancel.
+apply derives_refl'. f_equal. auto.
+Qed.
+
+
+Definition update_outer_if :=
+     Sifthenelse
+        (Ebinop One (Etempvar _n tuint) (Econst_int (Int.repr 0) tint) tint)
+        (Ssequence
+           (Sset _fragment
+              (Ebinop Osub
+                 (Ebinop Omul (Econst_int (Int.repr 16) tint)
+                    (Econst_int (Int.repr 4) tint) tint) (Etempvar _n tuint)
+                 tuint)) update_inner_if)
+        Sskip.
+
+Lemma update_outer_if_proof:
+ forall  (Espec : OracleKind) (hashed : list int) 
+           (dd data : list Z) (c d : val) (sh : share) (len : nat)
+   (H : len <= length data)
+   (HBOUND : (s256a_len (S256abs hashed dd) + Z.of_nat len * 8 < two_p 64)%Z)
+   (c' : name _c)
+   (data_ : name _data_)
+   (len' : name _len)
+   (data' : name _data)
+   (p : name _p)
+   (n : name _n)
+   (fragment : name _fragment)
+   (hi : int)
+   (lo : int)
+   (H7 : ((Zlength hashed * 4 + Zlength dd) * 8)%Z = hilo hi lo)
+   (H3 : length dd < CBLOCK)
+   (H3' : Forall isbyteZ dd) 
+   (H4 : NPeano.divide LBLOCK (length hashed))
+   (Hlen : (Z.of_nat len <= Int.max_unsigned)%Z),
+semax
+  (initialized _p
+     (initialized _n
+        (initialized _data (func_tycontext f_SHA256_Update Vprog Gtot))))
+  (PROP  ()
+   LOCAL 
+   (`eq (eval_id _p)
+      (`(deref_noload (tarray tuchar 64))
+         (`(offset_val (Int.repr (align 40 1))) (`force_ptr (eval_id _c))));
+   `(eq (Vint (Int.repr (Zlength dd)))) (eval_id _n);
+   `eq (eval_id _data) (eval_id _data_); `(eq c) (eval_id _c);
+   `(eq d) (eval_id _data_);
+   `((eq (Z.of_nat len) oo Int.unsigned) oo force_int) (eval_id _len))
+   SEP  (`(sha256_length (hilo hi lo + Z.of_nat len * 8) c);
+   `(array_at tuint Tsh
+       (ZnthV tuint (map Vint (process_msg init_registers hashed))) 0 8 c);
+   `(at_offset 40
+       (array_at tuchar Tsh (ZnthV tuchar (map Vint (map Int.repr dd))) 0 64)
+       c);
+   `(field_at Tsh t_struct_SHA256state_st _num (Vint (Int.repr (Zlength dd)))
+       c); K_vector; `(data_block sh data d))) update_outer_if
+  (overridePost (sha_update_inv sh hashed len c d dd data hi lo false)
+     (function_body_ret_assert tvoid
+        (EX  a' : s256abs,
+         PROP  (update_abs (firstn len data) (S256abs hashed dd) a')
+         LOCAL ()
+         SEP  (K_vector; `(sha256state_ a' c); `(data_block sh data d))))).
+Proof.
+intros.
+unfold update_outer_if.
+simplify_Delta; abbreviate_semax.
+unfold POSTCONDITION, abbreviate; clear POSTCONDITION.
+
+forward_if (sha_update_inv sh hashed len c d dd data hi lo false).
+* entailer!.   (* cond-expression typechecks *)
+* (* then clause *)
+forward.  (* fragment = SHA_CBLOCK-n; *)
+rewrite semax_seq_skip.
+
+apply semax_pre with (inv_at_inner_if sh hashed len c d dd data hi lo).
+unfold inv_at_inner_if; entailer!.
+rewrite H2.
+destruct (Int.unsigned_range_2 len'); auto.
+apply Int.repr_unsigned.
+fold (inv_at_inner_if sh hashed len c d dd data hi lo).
+apply semax_seq with (sha_update_inv sh hashed len c d dd data hi lo false).
+replace Delta with (initialized _fragment (initialized _p (initialized _n (initialized _data
+                     (func_tycontext f_SHA256_Update Vprog Gtot)))))
+ by (simplify_Delta; reflexivity).
+unfold POSTCONDITION, abbreviate; clear POSTCONDITION Delta.
+autorewrite with norm.
+apply (update_inner_if_proof Espec hashed dd data c d sh len hi lo); assumption.
+forward. 
+rewrite overridePost_normal'. apply andp_left2; auto.
+* (* else clause *)
+forward.  (* skip; *)
+rewrite overridePost_normal'.
+apply exp_right with nil. rewrite <- app_nil_end.
+entailer.
+ rewrite negb_false_iff in H1;  apply int_eq_e in H1.
+assert (Int.unsigned (Int.repr (Zlength dd)) = Int.unsigned (Int.repr 0)) by (f_equal; auto).
+rewrite (Int.unsigned_repr 0) in H6 by repable_signed.
+rewrite Int.unsigned_repr in H6 
+ by (clear - H3;
+      assert (Zlength dd < 64)%Z
+      by (rewrite Zlength_correct; change 64%Z with (Z.of_nat 64);
+       apply Nat2Z.inj_lt; assumption);
+      split; [rewrite Zlength_correct; omega | repable_signed]).
+rewrite Zlength_correct in H6; destruct dd; inv H6.
+ apply andp_right; [apply prop_right; repeat split | ].
+ + exists 0; reflexivity.
+ +  rewrite NPeano.Nat.sub_0_r, H2.
+   apply Int.repr_unsigned.
+ + rewrite <- app_nil_end. cancel.
+Qed.
+
+Lemma update_while_proof:
+ forall (Espec : OracleKind) (hashed : list int) (dd data: list Z)
+    (c d : val) (sh : share) (len : nat) 
+  (H : len <= length data)
+  (HBOUND : (s256a_len (S256abs hashed dd) + Z.of_nat len * 8 < two_p 64)%Z)
+  (c' : name _c) (data_ : name _data_) (len' : name _len)  
+  (data' : name _data) (p : name _p) (n : name _n)  (fragment : name _fragment)
+  (hi lo : int)
+  (H7 : ((Zlength hashed * 4 + Zlength dd) * 8)%Z = hilo hi lo)
+  (H3 : length dd < CBLOCK)
+  (H3' : Forall isbyteZ dd) 
+  (H4 : NPeano.divide LBLOCK (length hashed)) 
+  (Hlen : (Z.of_nat len <= Int.max_unsigned)%Z),
+ semax
+  (update_tycon
+     (initialized _p
+        (initialized _n
+           (initialized _data (func_tycontext f_SHA256_Update Vprog Gtot))))
+     update_outer_if) (sha_update_inv sh hashed len c d dd data hi lo false)
+  (Swhile
+     (Ebinop Oge (Etempvar _len tuint)
+        (Ebinop Omul (Econst_int (Int.repr 16) tint)
+           (Econst_int (Int.repr 4) tint) tint) tint) sha_update_loop_body)
+  (normal_ret_assert (sha_update_inv sh hashed len c d dd data hi lo true)).
+Proof.
+intros.
+simplify_Delta; abbreviate_semax.
+unfold POSTCONDITION, abbreviate; clear POSTCONDITION.
+apply semax_while.
++ reflexivity.
++ entailer!.
++ rewrite normal_ret_assert_elim.
+  unfold sha_update_inv.
+  normalize.
+  rewrite andp_assoc; do 2 rewrite insert_local.
+  apply exp_right with blocks.
+  entailer.
+
+  rename H5 into Hblocks;  assert (Hblocks' := Hblocks_lem Hblocks).
+  apply prop_right.
+  change (Int.mul (Int.repr 16) (Int.repr 4)) with (Int.repr 64) in H6;
+  rewrite negb_false_iff in H6;
+  apply Int.ltu_inv in H6.  
+  rewrite Int.unsigned_repr in H6.
+  destruct H6 as [_ H6].
+  apply Nat2Z.inj_lt;  apply H6.
+  split; [ clear; omega | ].
+  rewrite Nat2Z.inj_sub by auto.
+ omega.
++ unfold LOOP_BODY, abbreviate; clear LOOP_BODY.
+  unfold sha_update_inv at 1.
+  normalize.
+  apply extract_exists_pre; intro blocks.
+  rewrite insert_local.
+  apply semax_extract_PROP; apply intro_update_inv; intros.
+ apply (intro_PROP (Forall isbyteZ data /\ len - (length blocks*4 - length dd) >= CBLOCK));
+  [ | intros [BYTESdata Hlen_ge]]. {
+  rewrite (data_block_isbyteZ sh data d).
+  entailer!. rename H2 into H2'.
+  rewrite negb_true_iff in H1;
+   unfold Int.ltu in H1;
+  if_tac in H1; inv H1.
+  rewrite Int.unsigned_repr in H2;
+  change (Int.unsigned (Int.mul (Int.repr 16) (Int.repr 4)))
+    with (Z.of_nat CBLOCK) in H2.
+  apply Nat2Z.inj_ge.
+ apply H2.
+  split; [clear; omega | ].
+  rewrite Nat2Z.inj_sub by auto.
+  omega.
+}
+pose (bl := Zlist_to_intlist (firstn CBLOCK (skipn (length blocks * 4 - length dd) data) )).
+assert (H97: CBLOCK <= length (skipn (length blocks * 4 - length dd) data)). {
+rewrite skipn_length
+ by (clear - H Hblocks' Hblocks_len; omega).
+change (4*LBLOCK)%nat with CBLOCK.
+clear - Hlen_ge Hblocks' H Hblocks_len; omega.
+}
+assert (H1: length bl = LBLOCK). {
+unfold bl.
+apply length_Zlist_to_intlist.
+assert (H98: length data >= length blocks * 4 - length dd)
+ by (clear - H Hblocks' Hblocks_len; omega).
+rewrite firstn_length.
+apply min_l; auto.
+}
+assert (H0:  firstn CBLOCK (skipn (length blocks * 4 - length dd) data) =
+      intlist_to_Zlist bl). {
+unfold bl; rewrite Zlist_to_intlist_to_Zlist; auto.
+rewrite firstn_length.
+rewrite min_l by auto.
+exists LBLOCK; reflexivity.
+apply Forall_firstn.
+apply Forall_skipn; auto.
+}
+clearbody bl; clear H97.
+ simple apply (update_loop_body_proof Espec sh hashed dd data c d len (process_msg init_registers hashed) lo hi Delta blocks bl); 
+   try assumption.
+simplify_Delta; reflexivity.
+reflexivity.
+rewrite initial_world.Zlength_app.
+rewrite <- H7; f_equal.
+rewrite Zlength_intlist_to_Zlist.
+f_equal. apply Z.mul_comm.
+Qed.
